\section{Variance of EMA and relation to SMA}
Consider a white noise $X_t \sim \mathsf {i.i.d.} \Gaussian(0, 1)$ and two derived series.

For $Y_t = SMA_k(X_t) = \sum _{\tau=0}^{k-1} \frac{1}{k}X_{t-\tau}$ we have 
\begin{align}
	Var(Y_t) = \frac{1}{k} \label{eq:sma_variance}
\end{align}

On the other hand, for $Z_t = EMA_a(X_t) = (1-a)\sum_{\tau=0}^{\infty} a^{\tau} X_{t-\tau} = (1-a) X_t + a Z_{t-1}$ we have 
\begin{align}
Var(Z_t) = \frac{(1-a)^2}{1-a^2} = \frac{1-a}{1+a}	\label{eq:ema_variance}
\end{align}

Equating \autoref{eq:sma_variance} with \autoref{eq:ema_variance} we get a heuristic relation between parameters of SMA and EMA to achieve same level of smoothing
\begin{align} 
\boxed{a = \frac{k-1}{k+1}}
\end{align}.